src/Network.thy
@@ -19,13 +19,13 @@ lemma (in node_histories) node_total_order_trans:
   assumes "e1 \<sqsubset>\<^sup>i e2"
       and "e2 \<sqsubset>\<^sup>i e3"
     shows "e1 \<sqsubset>\<^sup>i e3"
-using assms
-  apply (clarsimp simp add: history_order_def)
-  apply (rule_tac x=xs in exI, rule_tac x="ys @ e2 # ysa" in exI, rule_tac x=zsa in exI)
-  apply (subgoal_tac "xs @ e1 # ys = xsa \<and> zs = ysa @ e3 # zsa")
+using assms unfolding history_order_def
   apply clarsimp
-  apply (rule_tac xs="history i" and ys="[e2]" in pre_suf_eq_distinct_list)
-  using histories_distinct apply auto
+  apply(rule_tac x=xs in exI, rule_tac x="ys @ e2 # ysa" in exI, rule_tac x=zsa in exI)
+  apply(subgoal_tac "xs @ e1 # ys = xsa \<and> zs = ysa @ e3 # zsa")
+  apply clarsimp
+  apply(rule_tac xs="history i" and ys="[e2]" in pre_suf_eq_distinct_list)
+  apply auto
 done
 
 lemma (in node_histories) local_order_carrier_closed:
@@ -36,7 +36,8 @@ using assms by (clarsimp simp add: history_order_def)
 
 lemma (in node_histories) node_total_order_irrefl:
   shows "\<not> (e \<sqsubset>\<^sup>i e)"
-by(clarsimp simp add: history_order_def) (metis Un_iff histories_distinct distinct_append distinct_set_notin list.set_intros(1) set_append)
+by(clarsimp simp add: history_order_def)
+  (metis Un_iff histories_distinct distinct_append distinct_set_notin list.set_intros(1) set_append)
 
 definition (in node_histories) prefix_of_node_history :: "'a list \<Rightarrow> nat \<Rightarrow> bool" (infix "prefix of" 50) where
   "xs prefix of i \<equiv> \<exists>ys. xs@ys = history i"
@@ -44,33 +45,42 @@ definition (in node_histories) prefix_of_node_history :: "'a list \<Rightarrow> 
 lemma (in node_histories) carriers_head_lt:
   assumes "y#ys = history i"
   shows   "\<not>(x \<sqsubset>\<^sup>i y)"
-using assms
+using assms unfolding history_order_def
   apply -
-  apply clarsimp
-  apply(subst (asm) history_order_def)
   apply clarsimp
   apply (subgoal_tac "xs @ x # ysa = [] \<and> zs = ys")
   apply clarsimp
   apply (rule_tac xs="history i" and ys="[y]" in pre_suf_eq_distinct_list)
-  using histories_distinct apply auto
+  apply auto
 done
 
-lemma (in node_histories) prefix_of_ConsD [dest]: "x # xs prefix of i \<Longrightarrow> [x] prefix of i"
-  by (auto simp: prefix_of_node_history_def)
+lemma (in node_histories) prefix_of_ConsD [dest]:
+  assumes "x # xs prefix of i"
+    shows "[x] prefix of i"
+using assms by(auto simp: prefix_of_node_history_def)
 
-lemma (in node_histories) prefix_of_appendD [dest]: "xs @ ys prefix of i \<Longrightarrow> xs prefix of i"
-  by (auto simp: prefix_of_node_history_def)
+lemma (in node_histories) prefix_of_appendD [dest]:
+  assumes "xs @ ys prefix of i"
+    shows "xs prefix of i"
+using assms by(auto simp: prefix_of_node_history_def)
 
-lemma (in node_histories) prefix_distinct: "xs prefix of i \<Longrightarrow> distinct xs"
-  apply (clarsimp simp: prefix_of_node_history_def)
-  by (metis histories_distinct distinct_append)
+lemma (in node_histories) prefix_distinct:
+  assumes "xs prefix of i"
+    shows "distinct xs"
+using assms by(clarsimp simp: prefix_of_node_history_def) (metis histories_distinct distinct_append)
 
-lemma (in node_histories) prefix_to_carriers [intro]: "xs prefix of i \<Longrightarrow> x \<in> set xs \<Longrightarrow> x \<in> set (history i)"
-  apply (clarsimp simp: prefix_of_node_history_def)
-  by (metis Un_iff set_append)
+lemma (in node_histories) prefix_to_carriers [intro]:
+  assumes "xs prefix of i"
+    shows "set xs \<subseteq> set (history i)"
+using assms by(clarsimp simp: prefix_of_node_history_def) (metis Un_iff set_append)
 
 lemma (in node_histories) local_order_prefix_closed:
-  "x \<sqsubset>\<^sup>i y \<Longrightarrow> xs prefix of i \<Longrightarrow> y \<in> set xs \<Longrightarrow> x \<in> set xs"
+  assumes "x \<sqsubset>\<^sup>i y"
+      and "xs prefix of i"
+      and "y \<in> set xs"
+    shows "x \<in> set xs"
+using assms
+  apply -
   apply (frule prefix_distinct)
   apply (insert histories_distinct[where i=i])
   apply (clarsimp simp: history_order_def prefix_of_node_history_def)
@@ -84,8 +94,8 @@ done
 
 lemma (in node_histories) local_order_prefix_closed_last:
   assumes "x \<sqsubset>\<^sup>i y"
-          "xs@[y] prefix of i"
-  shows   "x \<in> set xs"
+      and "xs@[y] prefix of i"
+    shows "x \<in> set xs"
 using assms
   apply -
   apply(frule local_order_prefix_closed, assumption, force)
@@ -95,10 +105,10 @@ done
 subsection\<open>Global order\<close>
 
 locale global_order = node_histories history for history :: "nat \<Rightarrow> 'a list" +
-  fixes global_order :: "'a \<Rightarrow> 'a \<Rightarrow> bool" (infix "\<sqsubset>\<^sup>G" 50)
-  assumes global_order_trans: "e1 \<sqsubset>\<^sup>G e2 \<Longrightarrow> e2 \<sqsubset>\<^sup>G e3 \<Longrightarrow> e1 \<sqsubset>\<^sup>G e3"
-   and local_order_to_global: "e1 \<sqsubset>\<^sup>i e2 \<Longrightarrow> e1 \<sqsubset>\<^sup>G e2"
-   and global_order_to_local: "{e1, e2} \<subseteq> set (history i) \<Longrightarrow> e1 \<sqsubset>\<^sup>G e2 \<Longrightarrow> e1 \<sqsubset>\<^sup>i e2"
+  fixes global_order :: "'a \<Rightarrow> 'a \<Rightarrow> bool" (infix "\<sqsubset>" 50)
+  assumes global_order_trans: "e1 \<sqsubset> e2 \<Longrightarrow> e2 \<sqsubset> e3 \<Longrightarrow> e1 \<sqsubset> e3"
+   and local_order_to_global: "e1 \<sqsubset>\<^sup>i e2 \<Longrightarrow> e1 \<sqsubset> e2"
+   and global_order_to_local: "{e1, e2} \<subseteq> set (history i) \<Longrightarrow> e1 \<sqsubset> e2 \<Longrightarrow> e1 \<sqsubset>\<^sup>i e2"
 
 subsection\<open>Networks\<close>
 
@@ -106,164 +116,140 @@ datatype 'a event
   = Broadcast 'a
   | Deliver 'a
 
-locale network = global_order history global_order for global_order :: "'a event \<Rightarrow> 'a event \<Rightarrow> bool" and history :: "nat \<Rightarrow> 'a event list" +
+locale network = global_order history global_order
+    for global_order :: "'a event \<Rightarrow> 'a event \<Rightarrow> bool" (infix "\<sqsubset>" 50) and history :: "nat \<Rightarrow> 'a event list" +
   (* Broadcast/Deliver interaction *)
-  assumes broadcast_before_delivery: "Broadcast m \<in> set (history i) \<Longrightarrow> (Broadcast m) \<sqsubset>\<^sup>G (Deliver m)"
-   and no_message_lost: "Broadcast m \<in> set (history i) \<Longrightarrow> Deliver m \<in> set (history j)"
-   and delivery_has_a_cause: "Deliver m \<in> set (history i) \<Longrightarrow> \<exists>j. Broadcast m \<in> set (history j)"
-   and broadcasts_unique: "i \<noteq> j \<Longrightarrow> Broadcast m \<in> set (history i) \<Longrightarrow> \<not> Broadcast m \<in> set (history j)"
+  assumes broadcast_before_delivery: "Broadcast m \<in> set (history i) \<Longrightarrow> (Broadcast m) \<sqsubset> (Deliver m)"
+      and no_message_lost: "Broadcast m \<in> set (history i) \<Longrightarrow> Deliver m \<in> set (history j)"
+      and delivery_has_a_cause: "Deliver m \<in> set (history i) \<Longrightarrow> \<exists>j. Broadcast m \<in> set (history j)"
+      and broadcasts_unique: "i \<noteq> j \<Longrightarrow> Broadcast m \<in> set (history i) \<Longrightarrow> Broadcast m \<notin> set (history j)"
 
 locale fifo_network = network +
-  assumes delivery_fifo_order: "{Deliver m1, Deliver m2} \<subseteq> set (history j) \<Longrightarrow> Broadcast m1 \<sqsubset>\<^sup>i Broadcast m2 \<Longrightarrow> Deliver m1 \<sqsubset>\<^sup>j Deliver m2"
-   and broadcast_fifo_order: "{Broadcast m1, Broadcast m2} \<subseteq> set (history i) \<Longrightarrow> Deliver m1 \<sqsubset>\<^sup>j Deliver m2 \<Longrightarrow> Broadcast m1 \<sqsubset>\<^sup>i Broadcast m2"
+  assumes delivery_fifo_order: "{Deliver m1, Deliver m2} \<subseteq> set (history j) \<Longrightarrow>
+      Broadcast m1 \<sqsubset>\<^sup>i Broadcast m2 \<Longrightarrow> Deliver m1 \<sqsubset>\<^sup>j Deliver m2"
+   and broadcast_fifo_order: "{Broadcast m1, Broadcast m2} \<subseteq> set (history i) \<Longrightarrow>
+      Deliver m1 \<sqsubset>\<^sup>j Deliver m2 \<Longrightarrow> Broadcast m1 \<sqsubset>\<^sup>i Broadcast m2"
 
 locale causal_network = fifo_network +
-   assumes broadcast_causal: "{Deliver m1, Deliver m2} \<subseteq> set (history j) \<Longrightarrow> Deliver m1 \<sqsubset>\<^sup>i Broadcast m2 \<Longrightarrow> Deliver m1 \<sqsubset>\<^sup>j Deliver m2"
+  assumes broadcast_causal: "{Deliver m1, Deliver m2} \<subseteq> set (history j) \<Longrightarrow>
+    Deliver m1 \<sqsubset>\<^sup>i Broadcast m2 \<Longrightarrow> Deliver m1 \<sqsubset>\<^sup>j Deliver m2"
 
 definition (in network) node_deliver_messages :: "'a event list \<Rightarrow> 'a list" where
   "node_deliver_messages cs \<equiv> List.map_filter (\<lambda>e. case e of Deliver m \<Rightarrow> Some m | _ \<Rightarrow> None) cs"
 
-lemma (in network) node_deliver_messages_empty [simp]: "node_deliver_messages [] = []"
-  by(auto simp add: node_deliver_messages_def List.map_filter_simps)
+lemma (in network) node_deliver_messages_empty [simp]:
+  shows "node_deliver_messages [] = []"
+by(auto simp add: node_deliver_messages_def List.map_filter_simps)
 
-lemma (in network) node_deliver_messages_append: "node_deliver_messages (xs@ys) = (node_deliver_messages xs)@(node_deliver_messages ys)"
-  by(auto simp add: node_deliver_messages_def map_filter_def)
+lemma (in network) node_deliver_messages_append:
+  shows "node_deliver_messages (xs@ys) = (node_deliver_messages xs)@(node_deliver_messages ys)"
+by(auto simp add: node_deliver_messages_def map_filter_def)
 
-lemma (in network) node_deliver_messages_Broadcast [simp]: "node_deliver_messages [Broadcast m] = []"
-  by (clarsimp simp: node_deliver_messages_def map_filter_def)
+lemma (in network) node_deliver_messages_Broadcast [simp]:
+  shows "node_deliver_messages [Broadcast m] = []"
+by(clarsimp simp: node_deliver_messages_def map_filter_def)
 
-lemma (in network) node_deliver_messages_Deliver [simp]: "node_deliver_messages [Deliver m] = [m]"
-  by (clarsimp simp: node_deliver_messages_def map_filter_def)
+lemma (in network) node_deliver_messages_Deliver [simp]:
+  shows "node_deliver_messages [Deliver m] = [m]"
+by(clarsimp simp: node_deliver_messages_def map_filter_def)
 
 lemma (in network) prefix_msg_in_history:
-  shows "es prefix of i \<Longrightarrow> m \<in> set (node_deliver_messages es) \<Longrightarrow> Deliver m \<in> set (history i)"
-  by (auto simp: node_deliver_messages_def map_filter_def split: event.split_asm)
+  assumes "es prefix of i"
+      and "m \<in> set (node_deliver_messages es)"
+    shows "Deliver m \<in> set (history i)"
+using assms
+  apply(auto simp: node_deliver_messages_def map_filter_def split: event.split_asm)
+  using prefix_to_carriers apply auto
+done
 
-subsection\<open>Causal Network\<close>
+definition (in network) hb :: "'a \<Rightarrow> 'a \<Rightarrow> bool" where
+  "hb m1 m2 \<equiv> (\<exists>i. Broadcast m1 \<sqsubset>\<^sup>i Broadcast m2 \<or> Deliver m1 \<sqsubset>\<^sup>i Broadcast m2)"
 
-locale network = finite_event_structure +
-  (* Broadcast/Deliver interaction *)
-  assumes broadcast_before_delivery: "(i, Broadcast, m) \<in> set (carriers i) \<Longrightarrow> (i, Broadcast, m) \<sqsubset>\<^sup>G (j, Deliver, m)"
-  assumes no_message_lost: "(i, Broadcast, m) \<in> set (carriers i) \<Longrightarrow> (j, Deliver, m) \<in> set (carriers j)"
-  assumes delivery_has_a_cause: "(i, Deliver, m) \<in> set (carriers i) \<Longrightarrow> \<exists>j. (j, Broadcast, m) \<in> set (carriers j)"
-  assumes delivery_fifo_order: "{(j, Deliver, m1), (j, Deliver, m2)} \<subseteq> set (carriers j) \<Longrightarrow> (i, Broadcast, m1) \<sqsubset>\<^sup>i (i, Broadcast, m2) \<Longrightarrow> (j, Deliver, m1) \<sqsubset>\<^sup>j (j, Deliver, m2)"
-  assumes broadcast_fifo_order: "{(i, Broadcast, m1), (i, Broadcast, m2)} \<subseteq> set (carriers i) \<Longrightarrow> (j, Deliver, m1) \<sqsubset>\<^sup>j (j, Deliver, m2) \<Longrightarrow> (i, Broadcast, m1) \<sqsubset>\<^sup>i (i, Broadcast, m2)" 
-  assumes broadcast_causal: "{(j, Deliver, m1), (j, Deliver, m2)} \<subseteq> set (carriers j) \<Longrightarrow> (i, Deliver, m1) \<sqsubset>\<^sup>i (i, Broadcast, m2) \<Longrightarrow> (j, Deliver, m1) \<sqsubset>\<^sup>j (j, Deliver, m2)"
-  assumes broadcasts_unique: "i \<noteq> j \<Longrightarrow> (i, Broadcast, m) \<in> set (carriers i) \<Longrightarrow> \<not> (j, Broadcast, m) \<in> set (carriers j)"
+definition (in network) weak_hb :: "'a \<Rightarrow> 'a \<Rightarrow> bool" where
+  "weak_hb m1 m2 \<equiv> hb m1 m2 \<or> m1 = m2"
 
-subsection\<open>Trivial models\<close>
-
-interpretation trivial_model: network "\<lambda>m. []" "\<lambda>e1 m e2. False" "\<lambda>e1 e2. False"
-  by standard auto
-
-interpretation non_trivial_model: network
-  "\<lambda>m. if m = 0 then [(0, Broadcast, id), (0, Deliver, id)] else [(m, Deliver, id)]"
-  "\<lambda>e1 m e2. m = 0 \<and> e1 = (0, Broadcast, id) \<and> e2 = (0, Deliver, id)"
-  "\<lambda>e1 e2. (\<exists>m. e1 = (0, Broadcast, id) \<and> e2 = (m, Deliver, id))"
-  apply standard
-  apply force
-  apply (case_tac "i=0"; clarsimp)
-  apply force
-  apply (rule iffI)
-  apply clarsimp
-  apply (rule_tac x="[]" in exI; force)
-  apply clarsimp
-  apply(case_tac xs; case_tac ys; case_tac zs; clarsimp)
-  by standard (case_tac "i = 0"; force)+
-
-subsection\<open>Connecting network with happens before locale.\<close>
-
-locale network_with_ops = network carriers
-  for carriers :: "nat \<Rightarrow> (nat \<times> event_type \<times> 'a) list" +
+locale network_with_ops = causal_network _ history
+  for history :: "nat \<Rightarrow> 'a event list" +
   fixes interp :: "'a \<Rightarrow> 'b \<rightharpoonup> 'b"
 
 context network_with_ops begin
 
-definition hb :: "'a \<Rightarrow> 'a \<Rightarrow> bool" where
-  "hb m1 m2 \<equiv> (\<exists>i. ((i, Broadcast, m1) \<sqsubset>\<^sup>i (i, Broadcast, m2) \<or>
-                  (i, Deliver, m1) \<sqsubset>\<^sup>i (i, Broadcast, m2)))"
-
-definition weak_hb :: "'a \<Rightarrow> 'a \<Rightarrow> bool" where
-  "weak_hb m1 m2 \<equiv> hb m1 m2 \<or> m1 = m2"
-
 sublocale hb: happens_before weak_hb hb
 proof
-  fix x y
+  fix x y :: "'a"
   show "hb x y = (weak_hb x y \<and> \<not> weak_hb y x)"
-  unfolding hb_def weak_hb_def
-    apply standard
-    apply(erule exE)
-    apply(erule disjE)
-    apply(rule conjI)
-    apply(rule disjI1)
-    apply(rule_tac x=i in exI, simp)
-    apply(rule notI)
-    apply(erule disjE)
-    apply(erule exE)
-    apply(erule disjE)
-    apply(case_tac "i=ia")
-    apply clarsimp
-    using node_total_order_irrefl node_total_order_trans
-      local_order_carrier_closed insert_subset apply blast
-    using broadcasts_unique apply(meson insert_subset local_order_carrier_closed)
-    apply(case_tac "i=ia")
-    apply clarsimp
-    using broadcast_before_delivery local_order_carrier_closed node_total_order_trans apply(smt finite_event_structure.global_order_to_local finite_event_structure_axioms insert_subset node_total_order_irrefl)
-    apply(drule local_order_carrier_closed)+
-    using broadcasts_unique apply(meson insert_subset)
-    apply(frule local_order_carrier_closed)
-    using node_total_order_irrefl apply simp
-    apply(frule local_order_carrier_closed; clarsimp)
-    apply(frule delivery_has_a_cause)
-    apply(frule broadcast_causal[rotated], clarsimp)
-    apply(rule conjI, assumption)
-    apply(rule no_message_lost, assumption)
-    apply(rule conjI)
-    apply(erule exE)
-    apply force
-    apply(erule exE)
-    apply(rule conjI)
-    apply clarsimp
-    apply(rule conjI)
-    apply(rule notI)
-    apply(frule local_order_carrier_closed)
-    apply(frule local_order_carrier_closed) back
-    apply(drule delivery_fifo_order[rotated], clarsimp)
-    apply(rule conjI, assumption, assumption)
-    using node_total_order_irrefl apply (meson insert_subset node_total_order_trans)
-    apply(rule notI)
-    using broadcast_before_delivery apply (meson global_order_to_local global_order_trans insert_subset local_order_carrier_closed local_order_to_global node_total_order_irrefl)
-    apply clarsimp
-    using node_total_order_irrefl apply blast
-    apply(erule conjE)
-    apply(erule disjE)
-    apply(erule exE)
-    apply clarsimp
-    apply(erule disjE)
-    apply force
-    apply force
-    apply clarsimp
-  done
+  proof(rule iffI; unfold hb_def weak_hb_def; clarsimp)
+    fix i :: "nat"
+    assume "Broadcast x \<sqsubset>\<^sup>i Broadcast y \<or> Deliver x \<sqsubset>\<^sup>i Broadcast y"
+    thus "(\<forall>i. \<not> Broadcast y \<sqsubset>\<^sup>i Broadcast x \<and> \<not> Deliver y \<sqsubset>\<^sup>i Broadcast x) \<and> y \<noteq> x"
+    proof
+      assume "Broadcast x \<sqsubset>\<^sup>i Broadcast y"
+      thus "(\<forall>i. \<not> Broadcast y \<sqsubset>\<^sup>i Broadcast x \<and> \<not> Deliver y \<sqsubset>\<^sup>i Broadcast x) \<and> y \<noteq> x"
+        by(metis global_order.global_order_trans global_order_axioms global_order_to_local
+            insert_subset local_order_carrier_closed local_order_to_global
+            network.broadcast_before_delivery network_axioms node_total_order_irrefl)
+    next
+      assume "Deliver x \<sqsubset>\<^sup>i Broadcast y"
+      thus "(\<forall>i. \<not> Broadcast y \<sqsubset>\<^sup>i Broadcast x \<and> \<not> Deliver y \<sqsubset>\<^sup>i Broadcast x) \<and> y \<noteq> x"  
+        by(meson broadcast_before_delivery global_order_to_local global_order_trans insert_subset
+            local_order_carrier_closed local_order_to_global node_total_order_irrefl)
+    qed
+  qed
 next
-  fix x
+  fix x :: "'a"
   show "weak_hb x x"
-  unfolding weak_hb_def by force
+    by(simp add: weak_hb_def)
 next
-  fix x y z
-  assume "weak_hb x y" "weak_hb y z"
-  thus "weak_hb x z"
-  unfolding weak_hb_def hb_def
-    apply -
-    apply safe
-    apply (metis (mono_tags, hide_lams) broadcasts_unique insert_subset local_order_carrier_closed node_total_order_trans)
-    apply (meson delivery_fifo_order insert_subset local_order_carrier_closed no_message_lost node_total_order_trans)
-    apply (metis (no_types, lifting) broadcasts_unique insert_subset local_order_carrier_closed node_total_order_trans)
-    apply (meson broadcast_causal delivery_has_a_cause insert_subset local_order_carrier_closed no_message_lost node_total_order_trans)
-    apply blast
-    apply blast
-  done
+  fix x y z :: "'a"
+  assume "weak_hb x y"
+     and "weak_hb y z"
+    thus "weak_hb x z"
+  proof(unfold weak_hb_def hb_def)
+    assume 1: "(\<exists>i. Broadcast x \<sqsubset>\<^sup>i Broadcast y \<or> Deliver x \<sqsubset>\<^sup>i Broadcast y) \<or> x = y"
+       and 2: "(\<exists>i. Broadcast y \<sqsubset>\<^sup>i Broadcast z \<or> Deliver y \<sqsubset>\<^sup>i Broadcast z) \<or> y = z"
+      show "(\<exists>i. Broadcast x \<sqsubset>\<^sup>i Broadcast z \<or> Deliver x \<sqsubset>\<^sup>i Broadcast z) \<or> x = z"
+    proof(rule disjE[OF 1]; rule disjE[OF 2]; clarsimp)
+      fix i j :: "nat"
+      assume "Broadcast x \<sqsubset>\<^sup>i Broadcast y \<or> Deliver x \<sqsubset>\<^sup>i Broadcast y"
+         and "Broadcast y \<sqsubset>\<^sup>j Broadcast z \<or> Deliver y \<sqsubset>\<^sup>j Broadcast z"
+         and "x \<noteq> z"
+       thus "\<exists>i. Broadcast x \<sqsubset>\<^sup>i Broadcast z \<or> Deliver x \<sqsubset>\<^sup>i Broadcast z" 
+         by(smt broadcasts_unique delivery_fifo_order delivery_has_a_cause global_order_to_local
+              insert_subset local_order_carrier_closed local_order_to_global
+              network.broadcast_before_delivery network_axioms no_message_lost node_total_order_trans)
+    qed
+  qed
 qed
 
 end
 
+section\<open>Example instantiations and interpretations\<close>
+
+interpretation trivial_node_histories: node_histories "\<lambda>m. []"
+  by standard auto
+
+interpretation trivial_global_order: global_order "\<lambda>m. []" "\<lambda>e1 e2. False"
+  by standard (auto simp add: trivial_node_histories.history_order_def)
+
+interpretation trivial_network: network "\<lambda>e1 e2. False" "\<lambda>m. []"
+  by standard auto
+
+interpretation non_trivial_node_histories: node_histories "\<lambda>m. if m = 0 then [Broadcast id, Deliver id] else [Deliver id]"
+  by standard auto
+
+interpretation non_trivial_global_order: global_order "\<lambda>m. if m = 0 then [Broadcast id, Deliver id] else [Deliver id]"
+                                                      "\<lambda>e1 e2. e1 = Broadcast id \<and> e2 = Deliver id"
+  apply standard
+  apply(auto simp add: non_trivial_node_histories.history_order_def)
+  apply(metis (no_types, lifting) append_is_Nil_conv butlast.simps(2) butlast_append append_Cons neq_Nil_conv append_Nil last_snoc)
+  apply(metis (no_types, lifting) append_is_Nil_conv butlast.simps(2) butlast_append append_Cons neq_Nil_conv append_Nil last_snoc)
+  apply(simp add: append_eq_Cons_conv)
+  using distinct_set_notin apply fastforce
+done
+
+interpretation non_trivial_network: network "\<lambda>e1 e2. e1 = Broadcast id \<and> e2 = Deliver id"
+                                            "\<lambda>m. if m = 0 then [Broadcast id, Deliver id] else [Deliver id]"
+  by standard (auto split: split_if_asm)
+
 end
+  
